Näidis.v
@@ -1,0 +1,100 @@
+Require Import Coq.Arith.PeanoNat.
+Require Import Coq.Bool.Bool.
+Require Import Coq.Lists.List.
+Require Extraction.
+
+Module Type T.
+Parameter V: Type.
+Parameter eq: V -> V -> bool.
+End T.
+
+Module Type SeqType (t:T) <: T.
+Definition V := list t.V.
+Parameter eq: V -> V -> bool.
+Parameter nil: V.
+Parameter cons: t.V -> V -> V.
+Parameter app: V -> V -> V.
+Parameter foldr: forall {B}, (t.V -> B -> B) -> B -> V -> B.
+End SeqType.
+
+Module NatT <: T.
+Definition V := nat.
+
+Fixpoint eq (x y: V): bool:=
+match x, y with
+| O, O => true
+| S x, S y => eq x y
+| _, _ => false
+end.
+End NatT.
+
+Module Type PairT (A:T) (B:T) <: T.
+Definition V := (A.V * B.V)%type.
+Parameter eq: V -> V -> bool.
+End PairT.
+
+Module PairTI (A:T) (B:T) : PairT (A) (B).
+Definition V := (A.V * B.V)%type.
+
+Definition eq (x y: V): bool:=
+match x, y with
+| (x1,x2), (y1,y2) => A.eq x1 y1 && B.eq x2 y2
+end.
+End PairTI.
+
+Module Algo (Tn:T) (Tp:PairT(Tn)(Tn)) (M: SeqType(Tp)).
+Definition rev(xs: M.V): M.V :=
+M.foldr (fun p xs => M.app xs (M.cons p M.nil)) M.nil xs.
+End Algo.
+
+Import ListNotations.
+Module RocqList (t:T) <: SeqType(t).
+Definition V := list t.V.
+Fixpoint eq (xs ys: V) :=
+match xs, ys with
+| [], [] => true
+| x::xs, y::ys => t.eq x y && eq xs ys
+| _, _ => false
+end.
+Definition nil: V := [].
+Definition cons (x: t.V) (xs: V) := x::xs.
+Fixpoint app (xs ys:V) :=
+match xs with
+| [] => ys
+| x::xs => x :: app xs ys
+end.
+Fixpoint foldr {B} (f: t.V -> B -> B) (a: B) (xs: V) :=
+match xs with
+| [] => a
+| x::xs => f x (foldr f a xs)
+end.
+End RocqList.
+
+Module Paar := PairTI(NatT)(NatT).
+Module Lst : SeqType(Paar).
+Module L := RocqList(Paar).
+Definition V := list Paar.V.
+Definition eq := L.eq .
+Definition nil := L.nil.
+Definition cons := L.cons.
+Definition app := L.app.
+Definition foldr {B}:= @L.foldr B.
+End Lst.
+
+Extract Constant Lst.nil => "[]".
+(* Extract Constant Lst.cons => "(::)". *)
+Extract Constant Lst.app => "(@)".
+Extract Constant Lst.foldr => "fun f a xs -> List.fold_right f xs a".
+Extract Constant Lst.eq => "fun xs ys -> xs = ys".
+Module A := Algo(NatT)(Paar)(Lst).
+
+Extract Inductive unit => "unit" [ "()" ].
+Extract Inductive bool => "bool" [ "true" "false" ].
+Extract Inductive prod => "(*)" [ "(,)" ].
+Extract Inductive list => "list" [ "[]" "(::)" ].
+
+Extract Inductive nat => int [ "0" "Stdlib.Int.succ" ].
+
+Extract Constant NatT.eq => "fun x y -> x = y".
+
+Recursive Extraction A.rev.
